WIP actions

src/3d/prelude/EverParse3d.Actions.fst
@@ -24,22 +24,20 @@ module LP = LowParse.Spec.Base
 module LPL = LowParse.Low.Base
 
 unfold
-let valid_pos
+let valid_len
   (#k: LP.parser_kind)
   (#t: Type)
   (p: LP.parser k t)
   (h: HS.mem)
   (sl: input_buffer_t)
-  (pos: nat)
-  (pos': nat)
+  (len: nat)
 : Tot prop
 = I.live sl h /\
   begin
     let s = I.get_remaining sl h in
-    pos <= Seq.length s /\
-    begin match LP.parse p (Seq.slice s pos (Seq.length s)) with
+    begin match LP.parse p s with
     | None -> False
-    | Some (_, len) -> pos' == pos + len
+    | Some (_, len') -> len == len'
     end
   end
 
@@ -63,7 +61,7 @@ let validate_with_action_t' (#k:LP.parser_kind) (#t:Type) (p:LP.parser k t) (inv
     loc_not_unused_in h `loc_includes` l /\
     address_liveness_insensitive_locs `loc_includes` l /\
     l `loc_disjoint` I.footprint sl /\
-    (allow_reading ==> U64.v startPosition <= Seq.length (I.get_remaining sl h))
+    U64.v startPosition + Seq.length (I.get_remaining sl h) <= I.length_all sl
   )
   (ensures fun h res h' ->
     I.live sl h' /\
@@ -72,10 +70,11 @@ let validate_with_action_t' (#k:LP.parser_kind) (#t:Type) (p:LP.parser k t) (inv
     inv sl h' /\
     begin if LPE.is_success res
     then
-      let pos = if allow_reading then U64.v startPosition else 0 in
       let s = I.get_remaining sl h in
-      valid_pos p h sl (U64.v res) /\
-      I.get_remaining sl h' == (if allow_reading then s else Seq.slice s (U64.v res) (Seq.length s))
+      let len = U64.v res - U64.v startPosition in
+      len >= 0 /\
+      valid_len p h sl len /\
+      I.get_remaining sl h' == (if allow_reading then s else Seq.slice s len (Seq.length s))
     else
       True
     end
@@ -118,7 +117,6 @@ let leaf_reader
     end
   ))
 
-
 inline_for_extraction
 noextract
 let validate_with_success_action' (name: string) #nz #wk (#k1:parser_kind nz wk) #t1 (#p1:parser k1 t1) (#inv1:_) (#l1:eloc) (#ar:_)
@@ -144,8 +142,8 @@ let validate_with_success_action' (name: string) #nz #wk (#k1:parser_kind nz wk)
 inline_for_extraction
 noextract
 let validate_drop_true
-   #nz #wk (#k:parser_kind nz wk) (#t:Type) (#p:parser k t) (#inv:slice_inv) (#l:eloc) (v: validate_with_action_t p inv l true)
-: Tot (validate_with_action_t p inv l false)
+   (#k:LP.parser_kind) (#t:Type) (#p:LP.parser k t) (#inv:slice_inv) (#l:eloc) (v: validate_with_action_t' p inv l true)
+: Tot (validate_with_action_t' p inv l false)
 = fun input startPosition ->
   let res = v input startPosition in
   if LPE.is_success res
@@ -160,8 +158,8 @@ let validate_drop_true
 inline_for_extraction
 noextract
 let validate_drop
-   #nz #wk (#k:parser_kind nz wk) (#t:Type) (#p:parser k t) (#inv:slice_inv) (#l:eloc) #allow_reading (v: validate_with_action_t p inv l allow_reading)
-: Tot (validate_with_action_t p inv l false)
+   (#k:LP.parser_kind) (#t:Type) (#p:LP.parser k t) (#inv:slice_inv) (#l:eloc) #allow_reading (v: validate_with_action_t' p inv l allow_reading)
+: Tot (validate_with_action_t' p inv l false)
 = if allow_reading
   then validate_drop_true v
   else v
@@ -200,22 +198,506 @@ let validate_ret
 
 #push-options "--z3rlimit 16"
 
+module LPC = LowParse.Spec.Combinators
+
 inline_for_extraction noextract
-let validate_pair'
+let validate_pair
        (name1: string)
        #nz1 (#k1:parser_kind nz1 WeakKindStrongPrefix) #t1 (#p1:parser k1 t1)
        (#inv1:_) (#l1:eloc) (#ar1:_) (v1:validate_with_action_t p1 inv1 l1 ar1)
        #nz2 #wk2 (#k2:parser_kind nz2 wk2) #t2 (#p2:parser k2 t2)
        (#inv2:_) (#l2:eloc) (#ar2:_) (v2:validate_with_action_t p2 inv2 l2 ar2)
-  : validate_with_action_t (p1 `parse_pair` p2) (conj_inv inv1 inv2) (l1 `eloc_union` l2) (ar1 && ar2)
+  : validate_with_action_t (p1 `parse_pair` p2) (conj_inv inv1 inv2) (l1 `eloc_union` l2) false
   = fun input startPosition ->
     let h = HST.get () in
+    LPC.nondep_then_eq p1 p2 (I.get_remaining input h);
     [@(rename_let ("positionAfter" ^ name1))]
-    let pos1 = v1 input startPosition in
+    let pos1 = validate_drop v1 input startPosition in
     let h1 = HST.get () in
     modifies_address_liveness_insensitive_unused_in h h1;
     if LPL.is_error pos1
     then
       pos1
     else
-      v2 input pos1
+      validate_drop v2 input pos1
+
+inline_for_extraction noextract
+let validate_dep_pair
+      (name1: string)
+      #nz1 (#k1:parser_kind nz1 _) #t1 (#p1:parser k1 t1)
+      #inv1 #l1 (v1:validate_with_action_t p1 inv1 l1 true) (r1: leaf_reader p1)
+      #nz2 #wk2 (#k2:parser_kind nz2 wk2) (#t2:t1 -> Type) (#p2:(x:t1 -> parser k2 (t2 x)))
+      #inv2 #l2 #ar2 (v2:(x:t1 -> validate_with_action_t (p2 x) inv2 l2 ar2))
+  : Tot (validate_with_action_t (p1 `parse_dep_pair` p2) (conj_inv inv1 inv2) (l1 `eloc_union` l2) false)
+  = fun input startPosition ->
+      let h = HST.get () in
+      LPC.parse_dtuple2_eq p1 p2 (I.get_remaining input h);
+      [@(rename_let ("positionAfter" ^ name1))]
+      let pos1 = v1 input startPosition in
+      let h1 = HST.get() in
+      if LPL.is_error pos1
+      then begin
+        pos1
+      end
+      else
+        [@(rename_let ("" ^ name1))]
+        let x = r1 input in
+        let h15 = HST.get () in
+        let _ = modifies_address_liveness_insensitive_unused_in h h15 in
+        validate_drop (v2 x) input pos1
+
+inline_for_extraction noextract
+let validate_dep_pair_with_refinement_and_action'
+      (name1: string)
+      (id1: field_id)
+      (#nz1: _) (#k1:parser_kind nz1 _) (#t1: _) (#p1:parser k1 t1)
+      (#inv1: _) (#l1: _) (v1:validate_with_action_t p1 inv1 l1 true) (r1: leaf_reader p1)
+      (f: t1 -> bool)
+      (#inv1': _) (#l1': _) (#b: _) (a:t1 -> action p1 inv1' l1' b bool)
+      (#nz2: _) (#wk2: _) (#k2:parser_kind nz2 wk2) (#t2:refine _ f -> Type) (#p2:(x:refine _ f) -> parser k2 (t2 x))
+      (#inv2: _) (#l2: _) (#ar2: _) (v2:(x:refine _ f -> validate_with_action_t (p2 x) inv2 l2 ar2))
+  : Tot (validate_with_action_t
+             ((p1 `LPC.parse_filter` f) `(parse_dep_pair #nz1)` p2)
+             (conj_inv inv1 (conj_inv inv1' inv2))
+             (l1 `eloc_union` (l1' `eloc_union` l2))
+             false)
+  =
+  fun input startPosition ->
+      let h0 = HST.get () in
+      LPC.parse_dtuple2_eq' #_ #_ (p1 `LPC.parse_filter` f) #_ #t2 p2 (I.get_remaining input h0);
+      LPC.parse_filter_eq p1 f (I.get_remaining input h0);
+      [@(rename_let ("positionAfter" ^ name1))]
+      let res = v1 input startPosition in
+      let h1 = HST.get() in
+      modifies_address_liveness_insensitive_unused_in h0 h1;
+      if LPL.is_error res
+      then begin
+        res
+      end
+      else begin
+        assert (I.get_remaining input h1 == I.get_remaining input h0);
+        [@(rename_let ("" ^ name1))]
+        let field_value = r1 input in
+        [@(rename_let (name1 ^ "ConstraintIsOk"))]
+        let ok = f field_value in
+        [@(rename_let ("pos_or_error_after_" ^ name1))]
+        let res1 = check_constraint_ok_with_field_id ok startPosition res id1 in
+        if LPL.is_error res1
+        then
+          res1
+        else
+             let h2 = HST.get() in
+             modifies_address_liveness_insensitive_unused_in h1 h2;
+             if not (a field_value input)
+             then (LPL.set_validator_error_pos_and_code validator_error_action_failed startPosition id1) //action failed
+             else begin
+               let open LPL in
+               let h15 = HST.get () in
+               let _ = modifies_address_liveness_insensitive_unused_in h0 h15 in
+               validate_drop (v2 field_value) input res1
+             end
+        end
+
+inline_for_extraction noextract
+let validate_dep_pair_with_refinement_and_action_total_zero_parser'
+      (name1: string)
+      (id1: field_id)
+      (#nz1: _) (#k1:parser_kind nz1 WeakKindStrongPrefix) (#t1: _) (#p1:parser k1 t1) (r1: leaf_reader p1)
+      (inv1: _) (l1: _)
+      (f: t1 -> bool)
+      (#inv1': _) (#l1': _) (#b: _) (a:t1 -> action p1 inv1' l1' b bool)
+      (#nz2: _) (#wk2: _) (#k2:parser_kind nz2 wk2) (#t2:refine _ f -> Type) (#p2:(x:refine _ f -> parser k2 (t2 x)))
+      (#inv2: _) (#l2: _) (#ar2: _) (v2:(x:refine _ f -> validate_with_action_t (p2 x) inv2 l2 ar2))
+  : Pure (validate_with_action_t
+             ((p1 `LPC.parse_filter` f) `(parse_dep_pair #nz1)` p2)
+             (conj_inv inv1 (conj_inv inv1' inv2))
+             (l1 `eloc_union` (l1' `eloc_union` l2))
+             false)
+         (requires (
+           let open LP in
+           k1.parser_kind_high == Some 0 /\
+           k1.parser_kind_metadata == Some ParserKindMetadataTotal
+         ))
+         (ensures (fun _ -> True))
+  = fun input startPosition ->
+      let h0 = HST.get () in
+      LPC.parse_dtuple2_eq' #_ #_ (p1 `LPC.parse_filter` f) #_ #t2 p2 (I.get_remaining input h0);
+      LPC.parse_filter_eq p1 f (I.get_remaining input h0);
+      [@inline_let] let _ = LP.parser_kind_prop_equiv k1 p1 in
+      begin
+        LowStar.Comment.comment ("Validating field " ^ name1);
+        [@(rename_let ("" ^ name1))]
+        let field_value = r1 input in
+        [@(rename_let (name1 ^ "ConstraintIsOk"))]
+        let ok = f field_value in
+        [@(rename_let ("pos_or_error_after_" ^ name1))]
+        let res1 = check_constraint_ok_with_field_id ok startPosition startPosition id1 in
+        if LPL.is_error res1
+        then
+             res1
+        else let h2 = HST.get() in
+             modifies_address_liveness_insensitive_unused_in h0 h2;
+             if not (a field_value input)
+             then (LPL.set_validator_error_pos_and_code validator_error_action_failed startPosition id1) //action failed
+             else begin
+               let open LPL in
+               let h15 = HST.get () in
+               let _ = modifies_address_liveness_insensitive_unused_in h0 h15 in
+               validate_drop (v2 field_value) input res1
+             end
+        end
+
+inline_for_extraction noextract
+let validate_dep_pair_with_refinement_and_action
+      (p1_is_constant_size_without_actions: bool)
+      (name1: string)
+      (id1: field_id)
+      #nz1 (#k1:parser_kind nz1 _) #t1 (#p1:parser k1 t1)
+      #inv1 #l1 (v1:validate_with_action_t p1 inv1 l1 true) (r1: leaf_reader p1)
+      (f: t1 -> bool)
+      #inv1' #l1' #b (a:t1 -> action p1 inv1' l1' b bool)
+      #nz2 #wk2 (#k2:parser_kind nz2 wk2) (#t2:refine _ f -> Type) (#p2:(x:refine _ f -> parser k2 (t2 x)))
+      #inv2 #l2 #ar2 (v2:(x:refine _ f -> validate_with_action_t (p2 x) inv2 l2 ar2))
+  : Tot (validate_with_action_t ((p1 `parse_filter` f) `parse_dep_pair` p2)
+                                (conj_inv inv1 (conj_inv inv1' inv2))
+                                (l1 `eloc_union` (l1' `eloc_union` l2))
+                                false)
+  = if
+      p1_is_constant_size_without_actions `LP.bool_and`
+      (k1.LP.parser_kind_high = Some 0) `LP.bool_and`
+      (k1.LP.parser_kind_metadata = Some LP.ParserKindMetadataTotal)
+    then
+      validate_dep_pair_with_refinement_and_action_total_zero_parser' name1 id1 r1 inv1 l1 f a v2
+    else
+      validate_dep_pair_with_refinement_and_action' name1 id1 v1 r1 f a v2
+
+
+inline_for_extraction noextract
+let validate_dep_pair_with_action
+      #nz1 (#k1:parser_kind nz1 _) #t1 (#p1:parser k1 t1)
+      #inv1 #l1 (v1:validate_with_action_t p1 inv1 l1 true) (r1: leaf_reader p1)
+      #inv1' #l1' #b (a:t1 -> action p1 inv1' l1' b bool)
+      #nz2 #wk2 (#k2:parser_kind nz2 wk2) (#t2:t1 -> Type) (#p2:(x:t1 -> parser k2 (t2 x)))
+      #inv2 #l2 #ar2 (v2:(x:t1 -> validate_with_action_t (p2 x) inv2 l2 ar2))
+  : Tot (validate_with_action_t
+             (p1 `(parse_dep_pair #nz1)` p2)
+             (conj_inv inv1 (conj_inv inv1' inv2))
+             (l1 `eloc_union` (l1' `eloc_union` l2))
+             false)
+  = fun input startPosition ->
+      let h0 = HST.get () in
+      LPC.parse_dtuple2_eq' #_ #_ p1 #_ #t2 p2 (I.get_remaining input h0);
+      let res = v1 input startPosition in
+      let h1 = HST.get() in
+      modifies_address_liveness_insensitive_unused_in h0 h1;
+      if LPL.is_error res
+      then begin
+        res
+      end
+      else begin
+        let field_value = r1 input in
+        let h2 = HST.get() in
+        modifies_address_liveness_insensitive_unused_in h1 h2;
+        let action_result = a field_value input in
+        if not action_result
+        then validator_error_action_failed //action failed
+        else begin
+               let open LPL in
+               let h15 = HST.get () in
+               let _ = modifies_address_liveness_insensitive_unused_in h0 h15 in
+               validate_drop (v2 field_value) input res
+             end
+      end
+
+inline_for_extraction noextract
+let validate_dep_pair_with_refinement'
+      (name1: string)
+      (id1: field_id)
+      #nz1 (#k1:parser_kind nz1 _) #t1 (#p1:parser k1 t1)
+      #inv1 #l1 (v1:validate_with_action_t p1 inv1 l1 true) (r1: leaf_reader p1)
+      (f: t1 -> bool)
+      #nz2 #wk2 (#k2:parser_kind nz2 wk2) (#t2:refine _ f -> Type) (#p2:(x:refine _ f -> parser k2 (t2 x)))
+      #inv2 #l2 #ar2 (v2:(x:refine _ f -> validate_with_action_t (p2 x) inv2 l2 ar2))
+  : Tot (validate_with_action_t
+             ((p1 `LPC.parse_filter` f) `(parse_dep_pair #nz1)` p2)
+             (conj_inv inv1 inv2)
+             (l1 `eloc_union` l2)
+             false)
+  = fun input startPosition ->
+      let h0 = HST.get () in
+      LPC.parse_dtuple2_eq' #_ #_ (p1 `LPC.parse_filter` f) #_ #t2 p2 (I.get_remaining input h0);
+      LPC.parse_filter_eq p1 f (I.get_remaining input h0);
+      [@(rename_let ("positionAfter" ^ name1))]
+      let res = v1 input startPosition in
+      let h1 = HST.get() in
+      modifies_address_liveness_insensitive_unused_in h0 h1;
+      if LPL.is_error res
+      then begin
+        res
+      end
+      else begin
+        [@(rename_let ("" ^ name1))]
+        let field_value = r1 input in
+        [@(rename_let (name1 ^ "ConstraintIsOk"))]
+        let ok = f field_value in
+        [@(rename_let ("positionOrErrorAfter" ^ name1))]
+        let res1 = check_constraint_ok_with_field_id ok startPosition res id1 in
+        if LPL.is_error res1
+        then
+             res1
+        else let h2 = HST.get() in
+             // assert (B.modifies B.loc_none h1 h2);
+             // assert (inv1' input.LPL.base h2);
+             modifies_address_liveness_insensitive_unused_in h1 h2;
+             // assert (loc_not_unused_in h2 `loc_includes` l1');
+             let open LPL in
+             // assert (valid_pos (p1 `(LPC.parse_filter #k1 #t1)` f) h0 input (uint64_to_uint32 pos) (uint64_to_uint32 res));
+             let h15 = HST.get () in
+             let _ = modifies_address_liveness_insensitive_unused_in h0 h15 in
+             validate_drop (v2 field_value) input res1
+        end
+
+inline_for_extraction noextract
+let validate_dep_pair_with_refinement_total_zero_parser'
+      (name1: string)
+      (id1: field_id)
+      #nz1 (#k1:parser_kind nz1 _) #t1 (#p1:parser k1 t1)
+      (inv1: _) (l1: _) (r1: leaf_reader p1)
+      (f: t1 -> bool)
+      #nz2 #wk2 (#k2:parser_kind nz2 wk2) (#t2:refine _ f -> Type) (#p2:(x:refine _ f -> parser k2 (t2 x)))
+      #inv2 #l2 #ar2 (v2:(x:refine _ f -> validate_with_action_t (p2 x) inv2 l2 ar2))
+  : Pure (validate_with_action_t
+             ((p1 `LPC.parse_filter` f) `(parse_dep_pair #nz1)` p2)
+             (conj_inv inv1 inv2)
+             (l1 `eloc_union` l2)
+             false)
+         (requires (
+           let open LP in
+           k1.parser_kind_high == Some 0 /\
+           k1.parser_kind_metadata == Some ParserKindMetadataTotal
+         ))
+         (ensures (fun _ -> True))
+  = fun input startPosition ->
+      let h0 = HST.get () in
+      LPC.parse_dtuple2_eq' #_ #_ (p1 `LPC.parse_filter` f) #_ #t2 p2 (I.get_remaining input h0);
+      LPC.parse_filter_eq p1 f (I.get_remaining input h0);
+      [@inline_let] let _ = LP.parser_kind_prop_equiv k1 p1 in
+      begin
+        LowStar.Comment.comment ("Validating field " ^ name1);
+        [@(rename_let ("" ^ name1))]
+        let field_value = r1 input in
+        [@(rename_let (name1 ^ "ConstraintIsOk"))]
+        let ok = f field_value in
+        [@(rename_let ("positionOrErrorAfter" ^ name1))]
+        let res1 = check_constraint_ok_with_field_id ok startPosition startPosition id1 in
+        if LPL.is_error res1
+        then res1
+        else let h2 = HST.get() in
+             // assert (B.modifies B.loc_none h1 h2);
+             // assert (inv1' input.LPL.base h2);
+             modifies_address_liveness_insensitive_unused_in h0 h2;
+             // assert (loc_not_unused_in h2 `loc_includes` l1');
+             let open LPL in
+             // assert (valid_pos (p1 `(LPC.parse_filter #k1 #t1)` f) h0 input (uint64_to_uint32 pos) (uint64_to_uint32 res));
+             let h15 = HST.get () in
+             let _ = modifies_address_liveness_insensitive_unused_in h0 h15 in
+             validate_drop (v2 field_value) input res1
+        end
+
+inline_for_extraction noextract
+let validate_dep_pair_with_refinement
+      (p1_is_constant_size_without_actions: bool)
+      (name1: string)
+      (id1: field_id)
+      #nz1 (#k1:parser_kind nz1 _) #t1 (#p1:parser k1 t1)
+      #inv1 #l1 (v1:validate_with_action_t p1 inv1 l1 true) (r1: leaf_reader p1)
+      (f: t1 -> bool)
+      #nz2 #wk2 (#k2:parser_kind nz2 wk2) (#t2:refine _ f -> Type) (#p2:(x:refine _ f -> parser k2 (t2 x)))
+      #inv2 #l2 #ar2 (v2:(x:refine _ f -> validate_with_action_t (p2 x) inv2 l2 ar2))
+  : Tot (validate_with_action_t ((p1 `parse_filter` f) `parse_dep_pair` p2)
+                                (conj_inv inv1 inv2)
+                                (l1 `eloc_union` l2)
+                                false)
+  = if
+      p1_is_constant_size_without_actions `LP.bool_and`
+      (k1.LP.parser_kind_high = Some 0) `LP.bool_and`
+      (k1.LP.parser_kind_metadata = Some LP.ParserKindMetadataTotal)
+    then
+      validate_dep_pair_with_refinement_total_zero_parser' name1 id1 inv1 l1 r1 f v2
+    else
+      validate_dep_pair_with_refinement' name1 id1 v1 r1 f v2
+
+inline_for_extraction noextract
+let validate_filter (name: string) #nz (#k:parser_kind nz _) (#t:_) (#p:parser k t)
+                    #inv #l (v:validate_with_action_t p inv l true)
+                    (r:leaf_reader p) (f:t -> bool) (cr:string) (cf:string)
+  : Tot (validate_with_action_t #nz #WeakKindStrongPrefix (p `LPC.parse_filter` f) inv l false)
+  = fun input startPosition ->
+    let h = HST.get () in
+    LPC.parse_filter_eq p f (I.get_remaining input h);
+    [@(rename_let ("positionAfter" ^ name))]
+    let res = v input startPosition in
+    let h1 = HST.get () in
+    if LPL.is_error res
+    then res
+    else begin
+      LowStar.Comment.comment cr;
+      [@(rename_let ("" ^ name))]
+      let field_value = r input in
+      LowStar.Comment.comment (normalize_term ("start: " ^cf));
+      [@(rename_let (name ^ "ConstraintIsOk"))]
+      let ok = f field_value in
+      LowStar.Comment.comment (normalize_term ("end: " ^ cf));
+      check_constraint_ok ok res
+    end
+
+
+inline_for_extraction noextract
+let validate_filter_with_action
+                    (name: string) #nz (#k:parser_kind nz _) (#t:_) (#p:parser k t)
+                    #inv #l (v:validate_with_action_t p inv l true)
+                    (r:leaf_reader p) (f:t -> bool) (cr:string) (cf:string)
+                    (#b:bool) #inva (#la:eloc) (a: t -> action #nz #WeakKindStrongPrefix #(filter_kind k) #_ (p `LPC.parse_filter` f) inva la b bool)
+  : Tot (validate_with_action_t #nz #WeakKindStrongPrefix (p `LPC.parse_filter` f) (conj_inv inv inva) (eloc_union l la) false)
+  = fun input startPosition ->
+    let h = HST.get () in
+    LPC.parse_filter_eq p f (I.get_remaining input h);
+    [@(rename_let ("positionAfter" ^ name))]
+    let res = v input startPosition in
+    let h1 = HST.get () in
+    if LPL.is_error res
+    then res
+    else begin
+      LowStar.Comment.comment cr;
+      [@(rename_let ("" ^ name))]
+      let field_value = r input in
+      LowStar.Comment.comment (normalize_term ("start: " ^cf));
+      [@(rename_let (name ^ "ConstraintIsOk"))]
+      let ok = f field_value in
+      LowStar.Comment.comment (normalize_term ("end: " ^ cf));
+      if ok
+        then let h15 = HST.get () in
+             let _ = modifies_address_liveness_insensitive_unused_in h h15 in
+             if a field_value input
+             then res
+             else validator_error_action_failed
+      else validator_error_constraint_failed
+    end
+
+inline_for_extraction noextract
+let validate_with_dep_action
+                    (name: string) #nz (#k:parser_kind nz _) (#t:_) (#p:parser k t)
+                    #inv #l (v:validate_with_action_t p inv l true)
+                    (r:leaf_reader p)
+                    (#b:bool) #inva (#la:eloc) (a: t -> action p inva la b bool)
+  : Tot (validate_with_action_t #nz p (conj_inv inv inva) (eloc_union l la) false)
+  = fun input startPosition ->
+    let h = HST.get () in
+    [@(rename_let ("positionAfter" ^ name))]
+    let res = v input startPosition in
+    let h1 = HST.get () in
+    if LPL.is_error res
+    then res
+    else begin
+      [@(rename_let ("" ^ name))]
+      let field_value = r input in
+      let h15 = HST.get () in
+      let _ = modifies_address_liveness_insensitive_unused_in h h15 in
+      if a field_value input
+      then res
+      else validator_error_action_failed
+    end
+
+inline_for_extraction noextract
+let validate_weaken #nz #wk (#k:parser_kind nz wk) #t (#p:parser k t)
+                    #inv #l #ar (v:validate_with_action_t p inv l ar)
+                    #nz' #wk' (k':parser_kind nz' wk'{k' `is_weaker_than` k})
+  : Tot (validate_with_action_t (parse_weaken p k') inv l ar)
+  = fun input startPosition ->
+    let h = HST.get () in
+    v input startPosition
+
+
+/// Parser: weakening kinds
+
+inline_for_extraction noextract
+let validate_weaken_left (#nz:_) #wk (#k:parser_kind nz wk) (#t:_) (#p:parser k t)
+                         (#inv:_) (#l:_) #ar (v:validate_with_action_t p inv l ar)
+                         (#nz':_) #wk' (k':parser_kind nz' wk')
+  : validate_with_action_t (parse_weaken_left p k') inv l ar
+  = validate_weaken v (glb k' k)
+
+/// Parser: weakening kinds
+
+inline_for_extraction noextract
+let validate_weaken_right (#nz:_) #wk (#k:parser_kind nz wk) (#t:_) (#p:parser k t)
+                         (#inv:_) (#l:_) #ar (v:validate_with_action_t p inv l ar)
+                         (#nz':_) #wk' (k':parser_kind nz' wk')
+  : validate_with_action_t (parse_weaken_right p k') inv l ar
+  = validate_weaken v (glb k k')
+
+inline_for_extraction noextract
+let validate_impos ()
+  : Tot (validate_with_action_t (parse_impos ()) true_inv eloc_none true)
+  = fun _ _ -> validator_error_impossible
+
+inline_for_extraction noextract
+let validate_with_error
+  c v
+  = fun input startPosition ->
+    let endPositionOrError = v input startPosition in
+    LPL.maybe_set_error_code endPositionOrError startPosition c
+
+noextract inline_for_extraction
+let validate_ite
+  e p1 v1 p2 v2
+  = fun input startPosition ->
+      if e then validate_drop (v1 ()) input startPosition else validate_drop (v2 ()) input startPosition
+
+module LPLL = LowParse.Spec.List
+
+unfold
+let validate_list_inv
+  (#k: LPL.parser_kind)
+  (#t: Type)
+  (p: LPL.parser k t)
+  (inv: slice_inv)
+  (l: loc)
+  (g0 g1: Ghost.erased HS.mem)
+  (sl: input_buffer_t)
+  (pos0: U64.t)
+  (bpos: pointer U64.t)
+  (h: HS.mem)
+  (stop: bool)
+: GTot Type0
+= let h0 = Ghost.reveal g0 in
+  let h1 = Ghost.reveal g1 in
+  let pos1 = Seq.index (as_seq h bpos) 0 in
+  inv sl h0 /\
+  h `extends` h0 /\
+  loc_not_unused_in h0 `loc_includes` l /\
+  l `loc_disjoint` I.footprint sl /\
+  l `loc_disjoint` loc_buffer bpos /\
+  address_liveness_insensitive_locs `loc_includes` l /\
+  B.loc_buffer bpos `B.loc_disjoint` I.footprint sl /\
+  I.live sl h0 /\
+  I.live sl h /\
+  U64.v pos0 + Seq.length (I.get_remaining sl h0) <= I.length_all sl /\
+  live h1 bpos /\
+  modifies loc_none h0 h1 /\ (
+  if
+    LPL.is_error pos1
+  then
+    stop == true
+  else
+    U64.v pos0 <= U64.v pos1 /\
+    U64.v pos1 + Seq.length (I.get_remaining sl h) <= I.length_all sl /\
+    (valid (LPLL.parse_list p) h0 sl <==>
+     valid (LPLL.parse_list p) h sl) /\
+    (stop == true ==> Seq.length (I.get_remaining sl h) == 0)
+  ) /\
+  modifies (l `loc_union` loc_buffer bpos `loc_union` I.footprint sl) h1 h
+
+
+
+#pop-options
